examples/concordium-impls/src/lib.rs
@@ -1,20 +1,30 @@
 #![feature(register_tool, rustc_attrs)]
 #![register_tool(creusot)]
 #![feature(proc_macro_hygiene, stmt_expr_attributes)]
+// #![feature(use_attributes)]
 
+// #[cfg(feature = "hacspec_unsafe")]
+// use hacspec_lib::*;
+// use hacspec_attributes::*;
+
+#[cfg(creusot)]
+#[cfg(test)]
 extern crate creusot_contracts;
-
+#[cfg(creusot)]
+#[cfg(test)]
 use creusot_contracts::*;
 
 pub type Reject = i32;
 
-#[trusted]
+
+// #[cfg_attr(feature = "use_attributes", unsafe_hacspec)]
+#[cfg_attr(feature = "creusot", trusted)]
 // #[ensures(forall<n:i32> result <= n)]
 pub fn I32MIN () -> i32 {
     (!(0_i32)) ^ (((!(0_u32)) >> 1) as i32)
 }
 
-#[logic]
+#[cfg_attr(feature = "creusot", logic)]
 pub fn reject_impl_default() -> Reject {
     I32MIN ()
 }
@@ -25,7 +35,7 @@ pub enum OptionReject {
     NoneReject,
 }
 
-#[logic]
+#[cfg_attr(feature = "creusot", logic)]
 pub fn new_reject_impl(x : i32) -> OptionReject {
     if x < 0_i32 {
         OptionReject::SomeReject (x)
@@ -34,12 +44,12 @@ pub fn new_reject_impl(x : i32) -> OptionReject {
     }
 }
 
-#[logic]
+#[cfg_attr(feature = "creusot", logic)]
 pub fn reject_impl_convert_from_unit() -> Reject {
     I32MIN () + 1_i32
 }
 
-#[logic]
+#[cfg_attr(feature = "creusot", logic)]
 pub fn reject_impl_convert_from_parse_error() -> Reject {
     I32MIN () + 2_i32
 }
@@ -54,7 +64,7 @@ pub enum LogError {
     Malformed,
 }
 
-#[logic]
+#[cfg_attr(feature = "creusot", logic)]
 pub fn reject_impl_from_log_error(le: LogError) -> Reject {
     match le {
         LogError::Full => I32MIN () + 3_i32,
@@ -70,7 +80,7 @@ pub enum NewContractNameError {
     NewContractNameErrorInvalidCharacters,
 }
 
-#[logic]
+#[cfg_attr(feature = "creusot", logic)]
 pub fn reject_impl_from_new_contract_name_error(nre: NewContractNameError) -> Reject {
     match nre {
         NewContractNameError::NewContractNameErrorMissingInitPrefix => I32MIN () + 5_i32,
@@ -87,7 +97,7 @@ pub enum NewReceiveNameError {
     NewReceiveNameErrorInvalidCharacters,
 }
 
-#[logic]
+#[cfg_attr(feature = "creusot", logic)]
 pub fn reject_impl_from_new_receive_name_error(nre: NewReceiveNameError) -> Reject {
     match nre {
         NewReceiveNameError::NewReceiveNameErrorMissingDotSeparator => I32MIN () + 7_i32,
@@ -98,22 +108,22 @@ pub fn reject_impl_from_new_receive_name_error(nre: NewReceiveNameError) -> Reje
 
 pub type ContractState = u32;
 
-/// A type representing the constract state bytes.
-// #[derive(Default)]
-#[logic]
-pub fn try_from_u64_to_u32 (inp : i64) -> Result<u32, std::num::TryFromIntError> {
-    std::convert::TryFrom::try_from(inp)
-}
-#[logic]
-pub fn try_from_i64_to_u32 (inp : i64) -> Result<u32, std::num::TryFromIntError> {
-    std::convert::TryFrom::try_from(inp)
-}
-
-pub type SeekResult = Result<u64, ()>;
-// pub enum SeekResult {
-//     SeekResultOk (u64),
-//     SeekResultErr,
+// /// A type representing the constract state bytes.
+// // #[derive(Default)]
+// #[cfg_attr(feature = "test", logic)]
+// pub fn try_from_u64_to_u32 (inp : i64) -> Result<u32, std::num::TryFromIntError> {
+//     std::convert::TryFrom::try_from(inp)
 // }
+// #[cfg_attr(feature = "test", logic)]
+// pub fn try_from_i64_to_u32 (inp : i64) -> Result<u32, std::num::TryFromIntError> {
+//     std::convert::TryFrom::try_from(inp)
+// }
+
+// pub type SeekResult = Result<u64, ()>;
+pub enum SeekResult {
+    SeekResultOk (u64),
+    SeekResultErr (()),
+}
 
 #[derive(Copy, Clone)] // , Debug, PartialEq, Eq
 pub enum SeekFrom {
@@ -138,98 +148,98 @@ pub enum SeekFrom {
 pub type U32Option = Option<u32>;
 pub type I64Option = Option<i64>;
 
-#[trusted]
-pub fn contract_state_impl_seek(current_position :ContractState, pos: SeekFrom) -> (ContractState, SeekResult) { // (ContractState, SeekResult)    
+#[cfg_attr(feature = "creusot", trusted)]
+pub fn contract_state_impl_seek(current_position :ContractState, pos: SeekFrom) -> (ContractState, SeekResult) {
     match pos {
-        SeekFrom::Start (offset) => (offset as u32, SeekResult::Ok (offset)),
+        SeekFrom::Start (offset) => (offset as u32, SeekResult::SeekResultOk (offset)),
         SeekFrom::End(delta) => 
 	    if delta >= 0_i64 {
 		match current_position.checked_add(delta as u32) {
-		    U32Option::Some (b) => (b, SeekResult::Ok(delta as u64)),
-		    U32Option::None => (current_position, SeekResult::Err (())),
+		    U32Option::Some (b) => (b, SeekResult::SeekResultOk(delta as u64)),
+		    U32Option::None => (current_position, SeekResult::SeekResultErr (())),
 		}
 	    } else {
 		match delta.checked_abs() {
 		    I64Option::Some (b) => // {
 		    // let new_pos = 4_u32 - (b as u32);
-			((4_u32 - (b as u32)), SeekResult::Ok((4_u32 - (b as u32)) as u64)),
+			((4_u32 - (b as u32)), SeekResult::SeekResultOk((4_u32 - (b as u32)) as u64)),
 		    // }
-		    I64Option::None => (current_position, SeekResult::Err (())),
+		    I64Option::None => (current_position, SeekResult::SeekResultErr (())),
 		}
 	    },
         SeekFrom::Current(delta) => 
 	    if delta >= 0_i64 {
 		match current_position.checked_add(delta as u32) {
-		    U32Option::Some(offset) => (offset, SeekResult::Ok(offset as u64)),
-		    U32Option::None => (current_position, SeekResult::Err (())),
+		    U32Option::Some(offset) => (offset, SeekResult::SeekResultOk(offset as u64)),
+		    U32Option::None => (current_position, SeekResult::SeekResultErr (())),
 		}
 	    } else {
 		match delta.checked_abs() {
 		    I64Option::Some (b) => match current_position.checked_sub(b as u32) {
-			U32Option::Some(offset) => (offset, SeekResult::Ok(offset as u64)),
-			U32Option::None => (current_position, SeekResult::Err (())),
+			U32Option::Some(offset) => (offset, SeekResult::SeekResultOk(offset as u64)),
+			U32Option::None => (current_position, SeekResult::SeekResultErr (())),
 		    },
-		    I64Option::None => (current_position, SeekResult::Err (())),
+		    I64Option::None => (current_position, SeekResult::SeekResultErr (())),
 		}
 	    },
     }
 }
 
 // , load_state : &dyn Fn(*mut u8, u32, u32) -> ([u8], u32)
-#[trusted]
+#[cfg_attr(feature = "creusot", trusted)]
 pub fn contract_state_impl_read_read(current_position : ContractState, num_read: u32) -> (ContractState, usize) {
     (current_position + num_read, num_read as usize)
 }
 
 /// Read a `u32` in little-endian format. This is optimized to not
 /// initialize a dummy value before calling an external function.
-#[logic]
+#[cfg_attr(feature = "creusot", logic)]
 pub fn contract_state_impl_read_read_u64(current_position : ContractState, num_read : u32) -> (ContractState, bool) {
     (current_position + num_read, num_read == 8_u32)
 }
 
 /// Read a `u32` in little-endian format. This is optimized to not
 /// initialize a dummy value before calling an external function.
-#[logic]
+#[cfg_attr(feature = "creusot", logic)]
 pub fn contract_state_impl_read_read_u32(current_position : ContractState, num_read : u32) -> (ContractState, bool) {    
     (current_position + num_read, num_read == 4_u32)
 }
 
 /// Read a `u8` in little-endian format. This is optimized to not
 /// initialize a dummy value before calling an external function.
-#[logic]
+#[cfg_attr(feature = "creusot", logic)]
 pub fn contract_state_impl_read_read_u8(current_position : ContractState, num_read : u32) -> (ContractState, bool) {
     (current_position + num_read, num_read == 1_u32)
 }
 
-#[logic]
+#[cfg_attr(feature = "creusot", logic)]
 pub fn write_impl_for_contract_state_test(current_position : ContractState, len : u32) -> bool {
     current_position.checked_add(len).is_none() // Check for overflow
 }
-#[trusted]
+#[cfg_attr(feature = "creusot", trusted)]
 pub fn write_impl_for_contract_state(current_position : ContractState, num_bytes : u32) -> (ContractState, usize) {
     (current_position + num_bytes, num_bytes as usize)
 }
 
-#[logic]
+#[cfg_attr(feature = "creusot", logic)]
 pub fn has_contract_state_impl_for_contract_state_open() -> ContractState {
     0_u32
 }
 
-#[logic]
+#[cfg_attr(feature = "creusot", logic)]
 pub fn has_contract_state_impl_for_contract_state_reserve_0(len : u32, cur_size : u32) -> bool {
     cur_size < len
 }
-#[logic]
+#[cfg_attr(feature = "creusot", logic)]
 pub fn has_contract_state_impl_for_contract_state_reserve_1(res : u32) -> bool {
     res == 1_u32
 }
 
-#[logic]
+#[cfg_attr(feature = "creusot", logic)]
 pub fn has_contract_state_impl_for_contract_state_truncate_0(cur_size : u32, new_size : u32) -> bool {
     cur_size > new_size
 }
-#[logic]
+#[cfg_attr(feature = "creusot", logic)]
 pub fn has_contract_state_impl_for_contract_state_truncate_1(current_position : ContractState, new_size : u32) -> ContractState {
     if new_size < current_position {
 	new_size
@@ -240,7 +250,7 @@ pub fn has_contract_state_impl_for_contract_state_truncate_1(current_position : 
 
 pub type Parameter = u32;
 
-#[trusted]
+#[cfg_attr(feature = "creusot", trusted)]
 pub fn read_impl_for_parameter_read(current_position : Parameter, num_read : u32) -> (Parameter, usize) {
     (current_position + num_read, num_read as usize)
 }
@@ -248,13 +258,13 @@ pub fn read_impl_for_parameter_read(current_position : Parameter, num_read : u32
 // pub struct AttributeTag(pub u8);
 pub type AttributesCursor = (u32, u16);
 
-#[trusted]
+#[cfg_attr(feature = "creusot", trusted)]
 pub fn has_policy_impl_for_policy_attributes_cursor_next_test (policy_attribute_items : AttributesCursor) -> bool {
     let (_,remaining_items) = policy_attribute_items;
     remaining_items == 0_u16
 }
 
-#[trusted]
+#[cfg_attr(feature = "creusot", trusted)]
 pub fn has_policy_impl_for_policy_attributes_cursor_next_tag_invalid (policy_attribute_items : AttributesCursor, tag_value_len_1 : u8, num_read : u32) -> (AttributesCursor, bool) {
     let (current_position,remaining_items) = policy_attribute_items;
     let policy_attribute_items = (current_position + num_read, remaining_items);
@@ -262,7 +272,7 @@ pub fn has_policy_impl_for_policy_attributes_cursor_next_tag_invalid (policy_att
 }
 
 
-#[trusted]
+#[cfg_attr(feature = "creusot", trusted)]
 pub fn has_policy_impl_for_policy_attributes_cursor_next (policy_attribute_items : AttributesCursor, num_read : u32) -> AttributesCursor {
     let (current_position,remaining_items) = policy_attribute_items;
     (current_position + num_read, remaining_items - 1_u16)
